coq/denot/list_properties.v
@@ -1,0 +1,524 @@
+Require Import Coq.Logic.FunctionalExtensionality.
+Require Import Coq.Classes.RelationClasses.
+Require Coq.Relations.Relation_Definitions.
+Require Import Lia.
+
+Require Export lc.tactics.
+Require Import structures.Structures.
+Require Export structures.consistency.
+
+
+Import MonadNotation.
+Open Scope monad_scope.
+Import SetNotations.
+Local Open Scope set_scope.
+
+Fixpoint map2 {A B C} (f : A -> B -> C) (xs : list A) (ys : list B) : list C := 
+  match xs , ys with 
+  | x :: xs' , y :: ys' => f x y :: map2 f xs' ys' 
+  | _ , _ => nil
+  end.
+#[export] Hint Constructors List.Forall2 : core.
+
+
+Lemma Forall2_length {A} : forall f (l1 l2 : list A), List.Forall2 f l1 l2 -> length l1 = length l2.
+Proof.  induction 1; eauto. simpl. f_equal. auto. Qed.
+
+
+Definition monotone {A}{B} (F : P A -> P B) : Set := 
+  forall D1 D2, (D1 ⊆ D2) -> F D1 ⊆ F D2.
+
+(* aka sub_preserving *)
+Definition sub_reflecting {A}{B} (F : P A -> P B) : Set := 
+  forall D1 D2, F D1 ⊆ F D2 -> (D1 ⊆ D2).
+
+Definition finite {B} (X : P B) : Prop := 
+  exists E, (X ≃ mem E) /\ nonempty_fset E.
+
+
+Definition continuous {V}{A} (F : P V -> P A) : Set :=
+  forall X E, mem E ⊆ F X -> valid X 
+         -> exists D, (mem D ⊆ X) /\ ((mem E) ⊆ F (mem D)) /\ valid_mem D.
+
+
+
+(* ------------ environments ---------------------- *)
+
+Definition atoms := nat.
+Definition dom {A} : list A -> atoms := fun l => List.length l.
+Definition same_scope {A} (ρ1 ρ2 : list A) := dom ρ1 = dom ρ2.
+
+Fixpoint access {A} (d : A) (e : list A) (x : nat) : A :=
+  match e with 
+  | nil => d
+  | cons p e => 
+      match x with
+      | 0 => p
+      | S m => access d e m 
+      end
+  end.
+
+Fixpoint update {A} (n : nat) (D: A) (xs : list A) {struct xs} : list A := 
+  match xs with 
+  | nil => nil
+  | y :: ys => match n with 
+               | 0 => D :: ys
+               | S m => y :: update m D ys
+             end
+  end.
+
+Lemma access_fresh{A}{d}{ρ : list A}{x}:
+  not (x < dom ρ) ->
+  access d ρ x = d.
+Proof.
+  move: x.
+  induction ρ; simpl; intros x h; try done.
+  destruct x.
+  lia.
+  rewrite IHρ. lia. done. Qed.
+
+
+Lemma dom_update {A}{n:nat}{D:A}{xs:list A}: dom (update n D xs) = dom xs.
+Proof. move: n. 
+       induction xs; intro n; simpl; auto. 
+       destruct n; simpl; auto.
+Qed.
+
+#[export] Hint Rewrite (@dom_update) : rewr_list.
+
+
+Module EnvNotations.
+Notation "ρ ⋅ x" := (access (fun y => False) ρ x) (at level 50) : list_scope.
+Infix "⊆e" := (List.Forall2 Included) (at level 50) : list_scope.
+Infix "≃e" := (List.Forall2 Same_set) (at level 50) : list_scope.
+Infix "⊔e" := (map2 Union) (at level 60) : list_scope.
+End EnvNotations.
+
+Import EnvNotations.
+
+
+Section EnvProperties.
+
+Context {Value : Type}.
+
+Definition Rho V := list (P V).
+
+Definition Bottom : P Value := fun x => False.
+
+Definition monotone_env {A} (XS: atoms) (D : Rho Value -> P A) := 
+  forall ρ ρ' , dom ρ = XS -> ρ ⊆e ρ' -> (D ρ) ⊆ D ρ'.
+
+Definition finite_env : Rho Value -> Prop := List.Forall finite.
+  
+Definition nonempty_env : Rho Value -> Type := List.ForallT nonemptyT.
+
+Definition sub_env : Rho Value -> Rho Value -> Prop := List.Forall2 Included.
+
+Definition same_env : Rho Value -> Rho Value -> Prop := List.Forall2 Same_set.
+
+Definition continuous_In {A} (D:Rho Value -> P A) (ρ:Rho Value) (v:A) : Prop :=
+  v ∈ D ρ -> exists ρ' , exists (pf : finite_env ρ'),  ρ' ⊆e ρ /\ (v ∈ D ρ').
+
+Definition continuous_env {A} (D:Rho Value -> P A) (ρ:Rho Value) : Prop :=
+  forall (v : A), continuous_In D ρ v.
+
+Definition continuous_Sub {A} (D:Rho Value -> P A) (ρ:Rho Value) (V:fset A) : Prop :=
+  mem V ⊆ D ρ -> 
+  exists ρ', exists (pf : finite_env ρ'),
+    ρ' ⊆e ρ  /\ (mem V ⊆ D ρ').
+
+End EnvProperties.
+
+#[export] Instance Proper_same_env_dom {A} : Proper (same_env ==> Logic.eq) (@dom (P A)).
+Proof. 
+  intros x y S. unfold dom, same_env in *. eapply Forall2_length; eauto. Qed.
+
+#[export] Instance Proper_sub_env_dom {A} : Proper (sub_env ==> Logic.eq) (@dom (P A)).
+Proof. 
+  intros x y S. unfold dom, sub_env in *. eapply Forall2_length; eauto. Qed.
+
+#[export] Instance Proper_same_env_scope {A} : Proper (same_env ==> same_env ==> Logic.eq) (@same_scope (P A)).
+Proof. 
+  intros x1 y1 S1 x2 y2 S2. unfold same_scope in *. rewrite -> S1. rewrite -> S2. done. Qed.
+
+#[export] Instance Proper_sub_env_scope {A} : Proper (sub_env ==> sub_env ==> Logic.eq) (@same_scope (P A)).
+Proof. 
+  intros x1 y1 S1 x2 y2 S2. unfold same_scope in *. rewrite -> S1. rewrite -> S2. done. Qed.
+
+
+Section EnvResults.
+
+Context {Value : Type}.
+
+(* Nonempty environments *)
+
+Lemma extend_nonempty_env {ρ : Rho Value}{X} : 
+  nonemptyT X -> 
+  nonempty_env ρ -> nonempty_env (X :: ρ).
+Proof. intros NEP NEX. eapply List.ForallT_cons; eauto. Qed.
+
+
+Lemma join_finite_env {ρ1 ρ2 : Rho Value} : 
+  same_scope ρ1 ρ2 
+  -> finite_env ρ1
+  -> finite_env ρ2
+  -> finite_env (ρ1 ⊔e ρ2).
+Proof.
+  move: ρ2.
+  induction ρ1 as [| v1 r1].
+  all: intros ρ2 sc h1; destruct ρ2 as [| v2 r2]; intros h2; simpl; eauto.
+  inversion h1; subst; clear h1.
+  inversion h2; subst; clear h2.
+  econstructor; eauto. 
+  2: { 
+    eapply IHr1; eauto. inversion sc. auto.
+  } 
+  match goal with 
+  | [ H4 : finite v1 |- _ ] =>  destruct H4 as [E1 [s1 u1 ]] end.
+  match goal with 
+  | [ H4 : finite v2 |- _ ] =>  destruct H4 as [E2 [s2 u2 ]] end.
+  exists (union_fset E1 E2).
+  split.
+  rewrite -> s1.
+    rewrite -> s2.
+    rewrite union_mem. reflexivity.
+    eauto.
+Qed.
+
+Lemma join_lub {ρ ρ1 : Rho Value} :
+  ρ1 ⊆e ρ -> forall ρ2, ρ2 ⊆e ρ -> (ρ1 ⊔e ρ2) ⊆e ρ.
+Proof.
+  intro SS1.
+  induction SS1; intros ρ2 SS2; inversion SS2; subst.
+  simpl. auto.
+  simpl.
+  eapply List.Forall2_cons; eauto.
+  rewrite -> H3.
+  rewrite -> H.
+  rewrite union_idem.
+  reflexivity.
+Qed.
+  
+Lemma join_sub_left {ρ1 ρ2 : Rho Value} : 
+  same_scope ρ1 ρ2 ->
+  ρ1 ⊆e (ρ1 ⊔e ρ2).
+Proof.
+  move: ρ2.
+  induction ρ1; intros ρ2 h. 
+  - destruct ρ2; simpl; simpl in h; eauto.
+  - destruct ρ2; inversion h. 
+    econstructor. auto.
+    eapply IHρ1. eauto.
+Qed.
+
+Lemma join_sub_right {ρ1 ρ2 : Rho Value} : 
+  same_scope ρ1 ρ2 ->
+  ρ2 ⊆e (ρ1 ⊔e ρ2).
+Proof.
+  move: ρ2.
+  induction ρ1; intros ρ2 h. 
+  - destruct ρ2; inversion h. simpl; auto.
+  - destruct ρ2; inversion h. 
+    econstructor. auto.
+    eapply IHρ1. eauto.
+Qed.
+
+Definition initial_finite_env (ρ : Rho Value) (NE : nonempty_env ρ) : Rho Value.
+  induction NE. exact nil.
+  destruct p as [V _].
+  exact (cons ⌈ V ⌉ IHNE).
+Defined.
+
+Lemma initial_finite_dom : forall E NE, dom (initial_finite_env E NE) = dom E.
+Proof.
+  induction NE; simpl. auto.
+  destruct p as [v w].  simpl. congruence.
+Qed. 
+
+Lemma finite_singleton : forall {B} (v : B), finite ⌈ v ⌉.
+Proof. intros B v. exists (singleton_fset v).
+       repeat split; eauto. done. 
+Qed.
+
+
+
+Lemma initial_fin (ρ : Rho Value) (NE : nonempty_env ρ) :
+  finite_env (initial_finite_env ρ NE).
+Proof.
+  induction NE.
+  simpl. econstructor.
+  simpl. destruct p as [v w1 ].
+  econstructor; eauto.
+  eapply finite_singleton.
+Qed.
+
+Lemma initial_fin_sub (ρ : Rho Value) (NE : nonempty_env ρ) :
+  initial_finite_env ρ NE ⊆e ρ.
+Proof.
+  induction NE; simpl. econstructor.
+  destruct p as [v fx].
+  econstructor; auto.
+Qed.
+
+
+(* single-env maps x to D and any other variable y to something in ρ y. *)
+Definition single_env (x : nat) (D : P Value) (ρ : Rho Value) 
+  (NE : nonempty_env ρ) : Rho Value :=
+  update x D (initial_finite_env ρ NE).
+
+  
+Lemma single_fin { X x ρ NE } : 
+  finite X ->
+  finite_env (single_env x X ρ NE).
+Proof.
+  move: x. induction NE; intro FIN; unfold finite_env; eauto.
+  unfold single_env. cbn. econstructor.
+  unfold single_env. simpl. destruct p as [v1 v2].
+  destruct FIN eqn:EQ.
+  + subst. simpl.
+    econstructor; eauto.
+    eapply initial_fin. 
+  + simpl in *.
+    econstructor; eauto.
+    eapply finite_singleton.
+    eapply IHNE; eauto.
+Qed.
+
+
+
+
+Lemma single_sub { ρ x V } :
+  forall (NE : nonempty_env ρ),
+    V ⊆ ρ ⋅ x 
+  -> (single_env x V ρ NE) ⊆e ρ.
+Proof.
+  intros NE. 
+  move: x.
+  induction NE.
+  all: intros vpe Indom. 
+  + (* nil case *) cbn. eauto.
+    
+  + (* cons case *)
+    unfold single_env in *.
+    destruct p as [w h2]. simpl.
+    destruct vpe.
+    ++ simpl in *.
+       econstructor; eauto.
+       eapply initial_fin_sub. 
+    ++ simpl in *.
+       econstructor; eauto.
+Qed.
+
+
+
+Lemma update_access : forall {x ρ NE X},
+  x < dom ρ ->
+  X ≃ (single_env x X ρ NE) ⋅ x.
+Proof.
+  intros.
+  unfold single_env.
+  move: NE x H.
+  induction NE. intros x H. simpl in H. lia.
+  simpl. destruct p as [w h2]. simpl.
+  intros y H. destruct y eqn:EQ. subst. reflexivity.
+  specialize (IHNE n ltac:(lia)).
+  simpl.
+  auto.
+Qed.  
+
+
+
+(* v∈single[xv]x  *)
+Lemma v_single_xvx {v x ρ NE} : 
+  x < dom ρ ->
+  v ∈ (single_env x ⌈ v ⌉ ρ NE ⋅ x).
+Proof.
+  unfold single_env.
+  move: NE x.
+  induction NE; intros y h. simpl in h. lia.
+  simpl. destruct p as [w h2]. simpl.
+  destruct y. simpl. eauto.
+  simpl in *. eapply IHNE. lia.
+Qed.  
+
+(* continuous-∈⇒⊆ *)
+Lemma continuous_In_sub {A} (E : Rho Value -> (P A)) ρ (NE : nonempty_env ρ) :
+   monotone_env (dom ρ) E
+   -> forall V, mem V ⊆ E ρ
+   -> (forall v, v ∈ mem V -> continuous_In E ρ v)
+   -> exists ρ', exists (pf : finite_env ρ') ,  ρ' ⊆e ρ /\ (mem V ⊆ E ρ').
+Proof.
+  intros me VS.
+  eapply fset_induction with (f := VS).
+  Unshelve. 3: exact VS.
+  - move=> VE vcont.
+    exists (initial_finite_env ρ NE).
+    repeat split.
+    eapply (initial_fin ρ NE).
+    eapply initial_fin_sub; eauto. 
+    done.
+  - move=> a f IHVS VE vcont.
+    rewrite union_mem in VE.
+    destruct IHVS as [ ρ1 [ fρ1 [ ρ1ρ VEρ1 ]]]; eauto.
+    move=> v vIn. eapply vcont. rewrite union_mem. eapply Union_intror. auto.
+    destruct (vcont a) as [ρ2 [fρ2 [ρ2ρ VEρ2]]].
+    rewrite union_mem. econstructor; eauto. rewrite mem_singleton_eq. eauto.
+    eapply VE. econstructor; eauto. 
+    rewrite mem_singleton_eq. eauto.
+    exists (ρ1 ⊔e ρ2).
+    have S1: same_scope ρ1 ρ. admit.
+    have S2: same_scope ρ2 ρ. admit.
+    have SS: same_scope ρ1 ρ2. admit. 
+    eexists. eapply join_finite_env; eauto.
+    repeat split.
+    + eapply join_lub; eauto.
+    + intros d dm.
+      rewrite union_mem in dm.
+      rewrite mem_singleton_eq in dm.
+      inversion dm; subst.
+      eapply me with (ρ := ρ2). rewrite -> ρ2ρ. auto. 
+      eapply join_sub_right; eauto. inversion H. subst. auto.
+      eapply me with (ρ := ρ1). rewrite -> ρ1ρ. auto. eapply join_sub_left; eauto. auto.
+Admitted.
+
+
+Lemma access_continuous_env { ρ x } : 
+  nonempty_env ρ -> continuous_env (fun ρ0 : Rho Value => ρ0 ⋅ x) ρ.
+Proof. 
+  move=> NE v vIn.
+  cbn in vIn.
+  destruct (Nat.lt_decidable x (dom ρ)).
+  exists (single_env x ⌈ v ⌉ ρ NE).
+  repeat split.
+  eapply single_fin; eauto.
+  eapply finite_singleton; eauto.
+  eapply single_sub; auto.
+  eapply v_single_xvx; eauto.
+  exists (initial_finite_env ρ NE).
+  rewrite access_fresh in vIn. auto. done.
+Qed.
+
+(* ⟦⟧-continuous-⊆ *) 
+Lemma generic_continuous_sub {A}{ρ}{F : Rho Value -> P A} : 
+    continuous_env F ρ 
+  -> monotone_env (dom ρ) F
+  -> nonempty_env ρ
+  -> forall V, mem V ⊆ F ρ
+  -> exists ρ', exists (pf : finite_env ρ'),
+        ρ' ⊆e ρ  /\  (mem V ⊆ F ρ').
+Proof.
+  intros Fcont Fmono NE_ρ V VinEρ.
+  eapply continuous_In_sub; eauto.
+Qed.
+
+
+End EnvResults.
+
+#[export] Hint Resolve extend_nonempty_env : core.
+#[export] Hint Resolve single_sub : core. 
+#[export] Hint Resolve single_fin : core. 
+#[export] Hint Resolve initial_fin_sub : core. 
+#[export] Hint Resolve initial_fin : core. 
+#[export] Hint Resolve finite_singleton : core. 
+#[export] Hint Rewrite @initial_finite_dom : rewr_list.
+#[export] Hint Resolve v_single_xvx : core. 
+
+
+(* Sub environments ⊆e *)
+
+Section EnvCongruence.
+
+Context {Value : Type}.
+
+Lemma Reflexive_sub_env {ρ:list (P Value)} : ρ ⊆e ρ.
+Proof.
+  induction ρ; econstructor; eauto. reflexivity.
+Qed.
+
+Lemma extend_sub_env {ρ ρ': list (P Value)}{X} :
+  ρ ⊆e ρ' -> (X :: ρ) ⊆e (X :: ρ' ).
+Proof. intros; econstructor; eauto. reflexivity. Qed.
+
+Lemma access_mono_sub : forall (ρ1 ρ2 : list (P Value)) (x : nat),
+   ρ1 ⊆e ρ2 ->
+   ρ1 ⋅ x ⊆ ρ2 ⋅ x.
+intros. 
+destruct (Nat.lt_decidable  x (dom ρ1)).
+Admitted.
+(*
++ apply Forall2_access with (f := Included); auto.
+    + rewrite access_fresh. auto.
+      rewrite access_fresh. erewrite Forall2_dom in H0; eauto.
+      reflexivity.
+Qed.  *)
+
+Lemma same_env_sub_env : forall (x y : list (P Value)), x ≃e y <-> (x ⊆e y) /\ (y ⊆e x).
+Proof. 
+intros x y. split.
+induction 1. split; eauto. 
+move: H => [r1 r2].
+move: IHForall2 => [h1 h2]. 
+split; econstructor; eauto.
+intros [h1 h2]. 
+induction h1. eauto.
+inversion h2. subst.
+econstructor; eauto.
+split; auto.
+Qed. 
+
+
+End EnvCongruence.
+
+
+#[export] Instance Proper_access_sub {Value} : 
+  Proper (sub_env ==> Logic.eq ==> Included) (@access (P Value) (fun x => False)). 
+Proof.
+  intros x2 y2 S2 x3 y3 ->. eapply access_mono_sub. eauto.
+Qed.  
+
+#[export] Instance Proper_access_eq {Value} : 
+  Proper (same_env ==> Logic.eq ==> Same_set) (@access (P Value) (fun x => False)). 
+Proof.
+  intros x2 y2 EQ x3 y3 ->. 
+  apply same_env_sub_env in EQ. destruct EQ as [S1 S2].
+  split; eapply access_mono_sub; eauto.  
+Qed.  
+
+#[export] Instance Transitive_sub_env {Value}  : 
+  Transitive (@List.Forall2 (P Value) (P Value) Included).
+Proof. typeclasses eauto. Qed.
+
+#[export] Hint Resolve Reflexive_sub_env : core.
+#[export] Hint Resolve extend_sub_env : core.
+
+
+(* valid sets are inhabited *)
+Definition valid_is_nonempty {A} (V : P A) : valid V -> nonemptyT V := id.
+
+Lemma valid_join : forall {A} ( v1 v2 : P A), 
+    valid v1 -> 
+    valid v2 ->
+    valid (v1 ∪ v2).
+Proof.
+  intros A v1 v2 [x1 h1] [x2 h2].
+  exists x1. eapply Union_introl; eauto.
+Qed.
+
+Section ValidTheory.
+
+Context {Value : Type}.
+
+Lemma valid_nil : @nonempty_env Value nil.
+Proof. unfold nonempty_env. eauto. Qed.
+
+
+Lemma extend_valid_env {ρ : list (P Value)}{X} : 
+  valid X -> 
+  nonempty_env ρ -> nonempty_env (X :: ρ).
+Proof. intros NEP NEX. eapply List.ForallT_cons; eauto. Qed.
+
+End ValidTheory.
+
+#[export] Hint Resolve valid_nil : core.
+#[export] Hint Immediate valid_is_nonempty : core.
+#[export] Hint Resolve extend_valid_env : core.
